

Linear Algebra

Problem Set 2

1. * For the sake of contradiction, let us assume $\nexists B, B'$ such that $BA = I$ and $B'A = I$
- * Then corresponding to these left inverses of A , let $\exists C, C'$ such that $AC = I$ and $AC' = I$

(i) We prove that $B = C$ and $B' = C'$

$AC = I$	$AC' = I$
$B(AC) = B \cdot I$	$B'(AC') = B' \cdot I$
$(B \cdot A) \cdot C = B$	$(B'A) \cdot C' = B' \cdot I$
$I \cdot C = B$	$I \cdot C' = B'$
$C = B$	$C' = B'$

(ii) We now prove $B = B'$ and that our assumption was wrong
 $BA = AB = I$

$B'(AB) = B' \cdot I$	$B'A = AB' = I$
$(B' \cdot A) \cdot B = B'$	$B \cdot (AB') = B \cdot I$
$I \cdot B = B'$	$(BA) \cdot B' = B$
$B = B'$	$I \cdot B' = B$
	$B' = B$

* Thus, a matrix A can only have one unique left inverse

2. Consider the matrix $A_{m \times n} = \begin{bmatrix} a_{11} & a_{12} & a_{13} & \dots & a_{1n} \\ a_{21} & a_{22} & a_{23} & \dots & a_{2n} \\ \vdots & \vdots & \vdots & \ddots & \vdots \\ a_{m1} & a_{m2} & a_{m3} & \dots & a_{mn} \end{bmatrix}$, then the augmented

matrix A' corresponding to $AX = Y$ is as follows -

$$A'_{m \times (n+1)} = \begin{bmatrix} a_{11} & a_{12} & a_{13} & \dots & a_{1n} & y_1 \\ a_{21} & a_{22} & a_{23} & \dots & a_{2n} & y_2 \\ \vdots & \vdots & \vdots & \ddots & \vdots & \vdots \\ a_{m1} & a_{m2} & a_{m3} & \dots & a_{mn} & y_m \end{bmatrix}$$

We now discuss the 2 how to find A^{-1}

1) Let $A = \begin{bmatrix} 2 & -1 \\ 1 & 3 \end{bmatrix}$

Then $A' = \begin{bmatrix} 2 & -1 & | & y_1 \\ 1 & 3 & | & y_2 \end{bmatrix}$

R_1 is swapped with R_2 , $A' = \begin{bmatrix} 1 & 3 & | & y_2 \\ 2 & -1 & | & y_1 \end{bmatrix}$

$R_2 \leftarrow R_2 - 2R_1$, $A' = \begin{bmatrix} 1 & 3 & | & y_2 \\ 0 & -7 & | & y_1 - 2y_2 \end{bmatrix}$

$R_2 \leftarrow R_2 / (-7)$, $A' = \begin{bmatrix} 1 & 3 & | & y_2 \\ 0 & 1 & | & (y_1 - 2y_2)/(-7) \end{bmatrix}$

$R_1 \leftarrow R_1 - 3R_2$, $A' = \begin{bmatrix} 1 & 0 & | & (y_2 + 3y_1)/7 \\ 0 & 1 & | & (2y_2 - y_1)/7 \end{bmatrix}$, meaning A is invertible

$AX = Y \Rightarrow X = A^{-1}Y$, meaning

$$\begin{bmatrix} x_1 \\ x_2 \end{bmatrix} = \begin{bmatrix} (y_2 + 3y_1)/7 \\ (2y_2 - y_1)/7 \end{bmatrix} = \begin{bmatrix} \frac{3}{7} & \frac{1}{7} \\ -\frac{1}{7} & \frac{2}{7} \end{bmatrix} X \begin{bmatrix} y_1 \\ y_2 \end{bmatrix}$$

$\Rightarrow A^{-1} = \begin{bmatrix} \frac{3}{7} & \frac{1}{7} \\ -\frac{1}{7} & \frac{2}{7} \end{bmatrix}$

(ii) Let us consider $A = \begin{bmatrix} 1 & \frac{1}{2} & \frac{1}{3} \\ \frac{1}{2} & \frac{1}{3} & \frac{1}{4} \\ \frac{1}{3} & \frac{1}{4} & \frac{1}{5} \end{bmatrix}$

Take $A' = \begin{bmatrix} 1 & \frac{1}{2} & \frac{1}{3} & | & 1 & 0 & 0 \\ \frac{1}{2} & \frac{1}{3} & \frac{1}{4} & | & 0 & 1 & 0 \\ \frac{1}{3} & \frac{1}{4} & \frac{1}{5} & | & 0 & 0 & 1 \end{bmatrix}$

To get $A' = \begin{bmatrix} 1 & 0 & 0 & | & 9 & -36 & 30 \\ 0 & 1 & 0 & | & -36 & 192 & -180 \\ 0 & 0 & 1 & | & 30 & -180 & 180 \end{bmatrix}$

Thus, $A^{-1} = \begin{bmatrix} 9 & -36 & 30 \\ -36 & 192 & -180 \\ 30 & -180 & 180 \end{bmatrix}$

We apply the following operations in order:

- (a) $R_2 \leftarrow R_2 - \frac{1}{2}R_1$
- (b) $R_3 \leftarrow R_3 - \frac{1}{3}R_1$
- (c) $R_2 \leftarrow 12R_2$
- (d) $R_1 \leftarrow R_1 - \frac{R_2}{2}$
- (e) $R_3 \leftarrow 180R_3$
- (f) $R_2 \leftarrow R_2 - R_3$
- (g) $R_1 \leftarrow R_1 + \frac{1}{6}R_3$

3. The general procedure is as follows -

i) consider the augmented matrix A' ,

$$A'_{m \times (n+1)} = \left[\begin{array}{ccc|c} a_{11} & a_{12} & \dots & a_{1n} & y_1 \\ a_{21} & a_{22} & \dots & a_{2n} & y_2 \\ \vdots & \vdots & \ddots & \vdots & \vdots \\ a_{m1} & a_{m2} & \dots & a_{mn} & y_m \end{array} \right]$$

ii) Now, using row operations convert this matrix to a row reduced echelon matrix of the form $[I | Z]$.

iii) The solution is $X = Z$

Example : Take $A = \begin{bmatrix} 0 & 5 & -1 \\ 1 & 8 & -1 \\ 2 & 1 & 1 \end{bmatrix}$

$$A' = \begin{bmatrix} 0 & 5 & -1 & y_1 \\ 1 & 8 & -1 & y_2 \\ 2 & 1 & 1 & y_3 \end{bmatrix}$$

$R_1 \leftrightarrow R_2$

$$A' = \begin{bmatrix} 1 & 8 & -1 & y_2 \\ 0 & 5 & -1 & y_1 \\ 2 & 1 & 1 & y_3 \end{bmatrix}$$

$R_3 \leftarrow R_3 - 2R_1$

$$A' = \begin{bmatrix} 1 & 8 & -1 & y_2 \\ 0 & 5 & -1 & y_1 \\ 0 & -15 & 3 & y_3 - 2y_2 \end{bmatrix}$$

$R_2 \leftarrow R_2 / 5$

$$A' = \begin{bmatrix} 1 & 8 & -1 & y_2 \\ 0 & 1 & -1/5 & y_1/5 \\ 0 & -15 & 3 & y_3 - 2y_2 \end{bmatrix}$$

$R_2 \leftarrow R_2 - 8R_2$

$$A' = \begin{bmatrix} 1 & 0 & 2/5 & y_2 - 8y_1/5 \\ 0 & 1 & -1/5 & y_1/5 \\ 0 & -15 & 3 & y_3 - 2y_2 \end{bmatrix}$$

$$A' = \begin{bmatrix} 1 & 0 & 2/5 & y_2 - 8y_1/5 \\ 0 & 1 & -1/5 & y_1/5 \\ 0 & 0 & 0 & 0 \end{bmatrix}$$

Example: Take $A' = \begin{bmatrix} 0 & 5 & -1 & y_1 \\ 1 & 8 & -1 & y_2 \\ 2 & 1 & 1 & y_3 \end{bmatrix}$

We apply the following operations in order — (a) $R_1 \leftrightarrow R_2$

(b) $R_3 \leftarrow R_3 - 2R_1$

(c) $R_2 \leftarrow \frac{R_2}{5}$

(d) $R_1 \leftarrow R_1 - 5R_2$

(e) $R_3 \leftarrow R_3 + 15R_2$

$$\begin{pmatrix} 0 & 5 & -1 & y_1 \\ 1 & 8 & -1 & y_2 \\ 2 & 1 & 1 & y_3 \end{pmatrix} \rightarrow \begin{pmatrix} 1 & 8 & -1 & y_2 \\ 0 & 5 & -1 & y_1 \\ 2 & 1 & 1 & y_3 \end{pmatrix}$$

$$\begin{pmatrix} 1 & 8 & -1 & y_2 \\ 0 & 5 & -1 & y_1 \\ 0 & -15 & 3 & y_3 - 2y_2 \end{pmatrix}$$

$$\begin{pmatrix} 1 & 0 & 3/5 & y_2 - 8y_1/5 \\ 0 & 1 & -1/5 & y_1/5 \\ 0 & -15 & 3 & y_3 - 2y_2 \end{pmatrix}$$

$$\begin{pmatrix} 1 & 0 & 3/5 & y_2 - 8y_1/5 \\ 0 & 1 & -1/5 & y_1/5 \\ 0 & -15 & 3 & y_3 - 2y_2 \end{pmatrix}$$

$$\begin{pmatrix} 1 & 0 & 3/5 & y_2 - 8y_1/5 \\ 0 & 1 & -1/5 & y_1/5 \\ 0 & 0 & 0 & y_3 - 2y_2 + 3y_1 \end{pmatrix}$$

This implies the system is consistent iff $y_3 - 2y_2 + 3y_1 = 0$

$$\Rightarrow X = \begin{bmatrix} x_1 \\ x_2 \\ x_3 \end{bmatrix} = \begin{bmatrix} y_2 - \frac{8y_1}{5} \\ y_1/5 \\ 0 \end{bmatrix}$$

$$\Rightarrow x_1 = \frac{5y_2 - 8y_1}{5}$$

$$x_2 = \frac{y_1}{5}$$

$$x_3 = 0$$

From the above RREF,

we get —

(i) $x_1 + \frac{3}{5}x_3 = x_2 - \frac{8y_1}{5}$

(ii) $x_2 - \frac{x_3}{5} = \frac{y_1}{5}$

Taking $x_3 = c$, the solution set is —

$$\{x_1, x_2, x_3\} = \left\{ \frac{5y_2 - 8y_1}{5} + \frac{3c}{5}, \frac{y_1}{5} + \frac{c}{5}, c \right\}$$

4. (i) Let us prove $S_1 \Rightarrow S_2$

Given, matrix A is invertible

$$Ax = y$$

$$\Rightarrow x = A^{-1}y$$

$\Rightarrow Ax = y$ has a solution for every matrix $y_{n \times 1}$

(ii) Now let us prove $S_2 \Rightarrow S_1$

* Given, $Ax = y$ has a solution for every matrix $y_{n \times 1}$

$\Rightarrow Rx = z$ has a solution for every z

* It's then sufficient to show R is invertible, since $R \sim A$

$\{ R = (E_1 E_2 \dots E_s)A \text{ where } E_i \text{ is elementary matrix}$
 $\forall i \in [1, s] \}$

* Take $z_{n \times 1} = \begin{bmatrix} 0 \\ 0 \\ \vdots \\ 1 \end{bmatrix}$ $\{ \text{all 0's except last entry } 1 \}$

This $z_{n \times 1}$ must also have a solution

$\Rightarrow R$ cannot have a zero row

$\Rightarrow R$ is invertible

$\Rightarrow A$ is invertible

5. If matrix A is invertible, then

$$A E_1 E_2 E_3 \dots E_s = I$$

$$I = E_1 E_2 E_3 \dots E_s A, \text{ where } E_1, E_2 \dots E_s \text{ are elementary matrices}$$

* Now take $A = A_1 A_2 A_3 A_4 \dots A_k$

$$I = (E_1 E_2 E_3 \dots E_s A_1) (A_2 A_3 \dots A_k)$$

* Since the product is I , $(\prod_{i=1}^s E_i) A_1$ has a right inverse

$\Rightarrow (\prod_{i=1}^s E_i) A_1$ is invertible

$\Rightarrow A_1$ is invertible, since $\prod_{i=1}^s E_i$ is invertible

* We can repeat this procedure for any j by rewriting

$$A = (A_1 A_2 \dots A_{j-1}) A_j (A_{j+1} \dots A_k)$$

* Thus, $\forall j \in [1, k], A_j$ is invertible. Hence proved!

6. * Given, A is an invertible matrix and $\exists E_1, E_2 \in I, I$ such that

$$I = (E_1 E_2 E_3 \dots E_s) A$$

* Right-multiply A^{-1} , we get -

$$I \cdot A^{-1} = \left(\prod_{i=1}^s E_i \right) A \cdot A^{-1}$$

$$\Rightarrow A^{-1} = \left(\prod_{i=1}^s E_i \right) I$$

\Rightarrow The same sequence of operations when applied to I yields A^{-1} , hence proved!

7. * Take A^{-1} to be left inverse of A

$$\Rightarrow A^{-1}A = I$$

* Now consider $AX = 0$

$$\Rightarrow A^{-1}(AX) = A^{-1} \cdot 0$$

$$\Rightarrow (A^{-1}A) \cdot X = 0$$

$$\Rightarrow I \cdot X = 0$$

$$\Rightarrow X = 0$$

* Thus, $AX = 0$ has only trivial solutions. Hence proved!

8. * In a row-reduced echelon matrix, for all the non-zero rows, there exists a pivot element and this pivot element is 1

* The matrix is as below -

$$\begin{bmatrix} 0 & 0 & 0 & \dots & 1 & \dots & 0 & \dots & \dots & \dots & \dots \\ 0 & 0 & 0 & \dots & 0 & \dots & 1 & \dots & \dots & \dots & \dots \\ 0 & 0 & 0 & \dots & 0 & \dots & 0 & \dots & 1 & \dots & \dots \\ \vdots & & & & \vdots & & & & & & \vdots \end{bmatrix} \begin{matrix} u_1 \\ u_2 \\ u_3 \\ \vdots \end{matrix}$$

* Then, $\sum_{i=1}^n c_i u_i$ is of the form $\{c_1, c_2, c_3, \dots, c_n\}$, linear combination of u_i

* Since each c_i appears once individually $\forall i \in \{1, 2, 3, \dots, n\}$, and since $\sum_{i=1}^n c_i u_i = 0 \Rightarrow c_i = 0 \forall i \in \{1, 2, 3, \dots, n\}$

Thus, the given statement is true